Projection of a [[vector]] $b$ to the [[column space]] of [[matrix]] $A$
- $b - Ax$ has to be [[orthogonal]] to the [[column space]] of $A$
→ $A^\top \left(b-Ax\right) = 0$A^\top b
→ $A^\top b  = A^\top Ax$
→ $x  = \left(A^\top A \right)^{-1}A^\top b$

![[Pasted image 20221009111212.png]]


START
Basic
Projection of a [[vector]] $b$ to the [[column space]] of [[matrix]] $A$
Back: 
- $b - Ax$ has to be [[orthogonal]] to the [[column space]] of $A$
→ $A^\top \left(b-Ax\right) = 0$A^\top b
→ $A^\top b  = A^\top Ax$
→ $x  = \left(A^\top A \right)^{-1}A^\top b$

![[Pasted image 20221009111212.png]]
Tags: mathematics, linear algebra
<!--ID: 1665308790789-->
END