# definition inverse function
Given a [[function]] $f:X \rightarrow Y$ then $f^{-1}:Y \rightarrow X$ is the [[inverse function]] of $f$ if

$$
\forall x \in X: f^{-1}\left(f(x)\right) = x
$$
$$
\forall y \in Y: f\left(f^{-1}(y)\right) = y
$$


# anki
START
Basic
- definition [[inverse function]]
Back: 
Given a [[function]] $f:X \rightarrow Y$ then $f^{-1}:Y \rightarrow X$ is the [[inverse function]] of $f$ if

$$
\forall x \in X: f^{-1}\left(f(x)\right) = x
$$
$$
\forall y \in Y: f\left(f^{-1}(y)\right) = y
$$

Tags: mathematics
<!--ID: 1682941753044-->
END