[[series]] that arrises from the [[taylor series]] of a [[function]]
### [[power series]] 
$$
f(x) = \sum_{n=0}^\infty a_n (x-c)^n
$$
the constant c is often zero, resulting in:
$$
f(x) = \sum_{n=0}^\infty a_n x^n
$$


# anki
START
Basic
Definition of [[power series]]

Back:
[[series]] that arrises from the [[taylor series]] of a [[function]]
### [[power series]] 
$$
f(x) = \sum_{n=0}^\infty a_n (x-c)^n
$$
the constant c is often zero, resulting in:
$$
f(x) = \sum_{n=0}^\infty a_n x^n
$$


Tags: mathematics
<!--ID: 1690016269197-->
END